WIP low level spec

src/zksync_verifier.ec
@@ -1,6 +1,6 @@
 pragma Goals:printall.
 
-require import Logic UInt256 Memory YulPrimops Array.
+require import Logic UInt256 Memory YulPrimops Array Real.
 require import Utils.
 
 op p = W256.of_int 21888242871839275222246405745257275088696311157297823662689037894645226208583.
@@ -54,6 +54,151 @@ proof.
   progress.
   apply ConcretePrimops.apply_mstore_mload_same.
 qed.
+
+module PointNegate = {
+  proc low(point: uint256) : unit = {
+    var x, y;
+    x <@ Primops.mload(point);
+    y <@ Primops.mload(point + W256.of_int 32);
+    if (x = W256.zero /\ y = W256.zero) {
+      Primops.revert();
+    } else {
+      if (y <> W256.zero) {
+        Primops.mstore(point + W256.of_int 32, p - y);
+      }
+    }
+  }
+}.
+
+lemma pointNegate_actual_matches_low: equiv [
+    Test.pointNegate ~ PointNegate.low :
+    Primops.memory{1} = Primops.memory{2} /\
+      arg{1} = arg{2} /\
+    !Primops.reverted{1} /\
+    !Primops.reverted{2}
+      ==>
+        Primops.reverted{1} <=> Primops.reverted{2} /\
+        !Primops.reverted{1} =>
+        forall (idx: uint256),
+        Primops.memory{1}.[idx] =
+        Primops.memory{2}.[idx]
+    ].
+    proof.
+      exists* Primops.memory{1}.
+      elim*=>memory.
+      exists* point{1}.
+      elim*=>point.
+      proc.
+      case (ConcretePrimops.mload memory (point+W256.of_int 32) = W256.zero).
+      rcondt{1} 6.
+      progress.
+      wp.
+      call (ConcretePrimops.mload_spec memory (point + W256.of_int 32)).
+      wp.
+      skip.
+      progress.
+      case (ConcretePrimops.mload memory point = W256.zero).
+      rcondt{1} 8.
+      progress.
+      wp.
+      call (ConcretePrimops.mload_spec memory point).
+      wp.
+      call (ConcretePrimops.mload_spec memory (point + W256.of_int 32)).
+      wp.
+      skip.
+      progress.
+      inline Primops.revert.
+      rcondt{2} 3.
+      progress.
+      call (ConcretePrimops.mload_spec memory (point + W256.of_int 32)).
+      call (ConcretePrimops.mload_spec memory point).
+      skip.
+      progress.
+      wp.
+      progress.
+      inline Primops.mload.
+      wp.
+      skip.
+      progress.
+      rcondf{1} 8.
+      progress.
+      wp.
+      call (ConcretePrimops.mload_spec memory point).
+      wp.
+      call (ConcretePrimops.mload_spec memory (point + W256.of_int 32)).
+      wp.
+      skip.
+      progress.
+      rcondf{2} 3.
+      progress.
+      call (ConcretePrimops.mload_spec memory (point + W256.of_int 32)).
+      call (ConcretePrimops.mload_spec memory point).
+      skip.
+      progress.
+      rewrite H1 H2.
+      trivial.
+      wp.
+      rcondf{2} 3.
+      progress.
+      call (ConcretePrimops.mload_spec memory (point + W256.of_int 32)).
+      call (ConcretePrimops.mload_spec memory point).
+      skip.
+      progress.
+      inline Primops.mload.
+      wp.
+      skip.
+      progress.
+      rcondf{1} 6.
+      progress.
+      wp.
+      sp.
+      call (ConcretePrimops.mload_spec memory (point + W256.of_int 32)).
+      skip.
+      progress.
+      rcondf{2} 3.
+      progress.
+      call (ConcretePrimops.mload_spec memory (point + W256.of_int 32)).
+      call (ConcretePrimops.mload_spec memory point).
+      skip.
+      progress.
+      rewrite H1.
+      trivial.
+      rcondt{2} 3.
+      progress.
+      call (ConcretePrimops.mload_spec memory (point + W256.of_int 32)).
+      call (ConcretePrimops.mload_spec memory point).
+      skip.
+      progress.
+      sp.
+      sim.
+      inline Primops.mstore. (*TODO why doesn't call work here*)
+      sim.
+      inline Primops.mload.
+      wp.
+      skip.
+      progress.
+qed.
+      
+lemma pointNegate_low_correctness :
+    forall (x y point_addr : uint256),
+hoare [ PointNegate.low :
+    arg = point_addr /\
+    (x <> W256.zero \/ y <> W256.zero) /\
+        Primops.memory.[point_addr] = x /\
+        Primops.memory.[point_addr + (W256.of_int 32)] = y /\
+      y < p /\
+      Primops.reverted = false ==>
+    (
+        Primops.reverted = false =>
+    (
+        Primops.memory.[point_addr] = x /\
+        Primops.memory.[point_addr + (W256.of_int 32)] = (-y) %% p
+    )
+  )].
+proof.
+  admit.
+qed.
+
       
 lemma pointNegate_correctness :
     forall (x y point_addr : uint256),
@@ -62,15 +207,30 @@ hoare [ Test.pointNegate :
     (x <> W256.zero \/ y <> W256.zero) /\
         Primops.memory.[point_addr] = x /\
         Primops.memory.[point_addr + (W256.of_int 32)] = y /\
-        y < p ==>
+      y < p /\
+      Primops.reverted = false ==>
     (
         Primops.reverted = false =>
     (
         Primops.memory.[point_addr] = x /\
         Primops.memory.[point_addr + (W256.of_int 32)] = (-y) %% p
     )
-)]. proof.
-    progress.
+  )]. proof.
+      progress.
+      bypr.
+      move => &m h.
+      have low: Pr[PointNegate.low(arg{m}) @ &m :
+     ! (Primops.reverted = false =>
+        Primops.memory.[point_addr] = x /\
+      Primops.memory.[point_addr + (of_int 32)%W256] = (-y) %% p)] = 0%r.
+      admit.
+      rewrite - low.
+      byequiv pointNegate_actual_matches_low.
+      progress.
+      smt.
+      smt.
+      progress.
+      
     proc.
     simplify.
     inline Primops.mload Primops.mstore Primops.revert.
